current/colorConvStack.v
@@ -1,27 +1,5 @@
 Require Import ThreeSatReduction.   
 
-
-
-
-Theorem convertBaseColorable : forall i Gamma Delta G F eta S5 eta'' eta' C, 
-                                 setVertices Gamma C 0 eta' eta -> 
-                                 setCs eta' (3 * length Gamma) F eta'' eta -> 
-                                 genericUnique S5 (fun x => x) Delta -> 
-                                 convert_base Gamma Delta i G -> coloring eta' G C.
-Admitted. 
-
-Theorem colorWeakeningApp : forall eta1 eta2 eta3 G C,
-                           coloring (eta1++eta3) G C ->
-                           coloring (eta1++eta2++eta3) G C. 
-Proof.
-  intros. genDeps {{ eta2 }}. remember(eta1++eta3). induction H; intros. 
-  {constructor. }
-  {subst. econstructor. apply in_app_iff in H. inv H. auto. apply in_app_iff; simpl.
-   eauto. repeat rewrite in_app_iff. auto. apply in_app_iff in H0. inv H0; 
-   repeat rewrite in_app_iff; eauto. auto. auto. auto. eapply IHcoloring; eauto. }
-  {constructor; eauto. }
-Qed. 
-
 Theorem consApp : forall (A:Type) (hd:A) tl, hd::tl = [hd]++tl. auto. Qed. 
 Theorem plus0 : forall n, n = n + 0. auto. Qed. 
 
@@ -56,18 +34,6 @@ Qed.
 
 Theorem threeX : forall x, x+(x+(x+0)) = 3 * x + 0. auto. Qed. 
 
-Theorem helper : forall Gamma C p1 eta eta' i c G u eta'' v v0 u', 
-              u = getVar p1 -> setVertices Gamma C 0 eta' eta -> In (u,3*u,3*u+1,3*u+2) Gamma -> winner eta p1 u' ->
-              mkEdge i p1 (3*u) (3*u+1) (v,v0) -> In (3 * u', c) eta' -> 
-              coloring(eta' ++ (i,c)::eta'') G C ->
-              coloring(eta' ++ (i,c)::eta'') (newEdge v v0 G) C.
-Proof.
-  intros. inversion H3; subst. 
-  {inv H2. 
-   {copy H1. eapply V_V'MapToUOrC in H1; eauto. inv H1. 
-    {invertHyp. simpl in *. 
-Admitted. 
-
 Ltac tryInv := repeat (try inCons; try invertTupEq). 
 
 Theorem notInEta : forall Gamma C i c eta' epsilon eta u, setVertices Gamma C i eta' eta -> u < i -> 
@@ -85,35 +51,47 @@ Proof.
   {intros contra. inv contra. }
 Qed. 
 
-
-
-Theorem InTrueV : forall u c Gamma C i eta eta', setVertices Gamma C i eta' eta ->
-                                      In (3*u,c) eta' -> In (u, true) eta -> c = u /\ c < C.
+Theorem InTrueV : forall u c Gamma C i eta eta', 
+                    setVertices Gamma C i eta' eta -> In (3*u,c) eta' -> 
+                    In (u, true) eta -> c = u /\ c < C /\ In (3*u+1,C) eta'.
 Proof.
   intros. induction H. 
   {destruct (eq_nat_dec u u0). 
-   {tryInv; try omega; auto. negate H1. rewrite (plus0 (3*u0)).
-    eapply notInEta'; eauto. contradiction. }
-   {tryInv; try omega; auto. }
+   {tryInv; try (split;[auto|split;[omega|simpl;auto]]). omega. negate H1.
+    rewrite (plus0 (3*u0)). eapply notInEta'; eauto. contradiction. omega.
+    eapply IHsetVertices in H3; auto. invertHyp. split; auto. split. omega. simpl. 
+    eauto. }  
+   {tryInv; try omega; auto. eapply IHsetVertices in H1; eauto. invertHyp. split; auto.
+    split. omega. simpl. auto. }
   }
   {destruct (eq_nat_dec u u0). 
-   {tryInv; try omega; auto. negate H3. eapply notInEta; eauto. contradiction. }
-   {tryInv; try omega. auto. }
+   {tryInv; try omega; auto. negate H3. eapply notInEta; eauto. contradiction. 
+    eapply IHsetVertices in H3; eauto. invertHyp. split; auto. split. omega. 
+    simpl. auto. }
+   {tryInv; try omega. apply IHsetVertices in H3; auto. invertHyp. split; auto. 
+    split. omega. simpl. auto. }
   }
   {inv H0. }
 Qed. 
 
-Theorem InTrueV' : forall u Gamma C i eta eta', setVertices Gamma C i eta' eta ->
-                                       In (u, true) eta -> In (3*u+1, C) eta'.
+Theorem InFalseV : forall u c Gamma C i eta eta', 
+                    setVertices Gamma C i eta' eta -> In (3*u+1,c) eta' -> 
+                    In (u, false) eta -> c = u /\ u < C /\ In (3*u,C) eta'.
 Proof.
   intros. induction H. 
   {destruct (eq_nat_dec u u0). 
-   {tryInv; simpl;auto. }
-   {tryInv. omega. apply IHsetVertices in H2. simpl. eauto. }
+   {tryInv; try omega; auto. negate H3. eapply notInEta; eauto. contradiction. 
+    eapply IHsetVertices in H3; eauto. invertHyp. split; auto. split. omega. 
+    simpl. auto. }
+   {tryInv; try omega. apply IHsetVertices in H3; auto. invertHyp. split; auto. 
+    split. omega. simpl. auto. }
   }
   {destruct (eq_nat_dec u u0). 
-   {tryInv; simpl;auto. }
-   {tryInv. apply IHsetVertices in H2. simpl. eauto. }
+   {tryInv; try (split;[auto|split;[omega|simpl;auto]]); try omega. negate H1.
+    eapply notInEta'; eauto. contradiction. 
+    eapply IHsetVertices in H3; auto. invertHyp. split; auto. }
+   {tryInv; try omega; auto. eapply IHsetVertices in H1; eauto. invertHyp. split; auto.
+    split. omega. simpl. auto. }
   }
   {inv H0. }
 Qed. 
@@ -131,30 +109,93 @@ Proof.
   }
 Qed. 
 
+Theorem uniqueMid : forall (A:Type) D1 D2 (u:A) U, 
+                      genericUnique U (fun x => x) (D1++[u]++D2) ->
+                      ~ In u (D1++D2). 
+Proof.
+  induction D1; intros. 
+  {simpl in *. inv H. eapply genericUniqueNotIn. Focus 2. eauto. simpl. 
+   apply Union_intror. constructor. }
+  {inv H. rewrite consApp in H2. copy H2. eapply IHD1 in H2; eauto. simpl. 
+   intros c. inv c. eapply genericUniqueNotIn in H. Focus 2. apply Union_intror. 
+   constructor. apply H. rewrite in_app_iff. right. simpl. auto. contradiction. }
+Qed. 
+
+Theorem notInApp : forall (A:Type) D1 D2 (u u':A), ~ In u (D1++[u']++D2) ->
+                                              ~ In u (D1++D2). 
+Proof.
+  intros. rewrite in_app_iff in *. intros c. apply H. inv c. auto. right.
+  simpl. auto. 
+Qed. 
+
+
+Ltac invIn := 
+  match goal with
+      |H:In ?u (?x++?y) |- _ => rewrite in_app_iff in H; inv H; try invIn
+  end. 
+
+Ltac solveIn :=
+  match goal with
+      | |- In ?x (?a ++ ?b) => rewrite in_app_iff; 
+                            solve[left; solveIn|right; solveIn]
+      | |- In ?a ?b \/ In ?c ?d => simpl in *; solve[left; solveIn | right; solveIn]
+      | |- In ?a (?b::?c) => simpl; solve[left; auto|right; solveIn]
+      | |- _ => eauto
+  end. 
+
+Theorem TripleNotIn : forall (A:Type) (u1 u2 u3:A) U D1 D2 D3 D4, 
+                        genericUnique U (fun x => x) (D1++u1::D2++u2::D3++u3::D4) ->
+                        ~ In u1 (D1++D2++D3++D4) /\ ~ In u2 (D1++D2++D3++D4) /\
+                        ~ In u3 (D1++D2++D3++D4). 
+Proof.
+  intros. assert(D1++u1::D2++u2::D3++u3::D4=D1++[u1]++(D2++u2::D3++u3::D4)). 
+  auto. copy H. rewrite H0 in H. apply uniqueMid in H; eauto. 
+  assert(D1++u1::D2++u2::D3++u3::D4=(D1++u1::D2)++[u2]++(D3++u3::D4)). 
+  simpl. rewrite <- app_assoc. auto. copy H1. rewrite H2 in H1. 
+  eapply uniqueMid in H1. 
+  assert(D1++u1::D2++u2::D3++u3::D4=(D1++u1::D2++u2::D3)++[u3]++D4). simpl.
+  rewrite <- app_assoc. simpl. rewrite <- app_assoc. auto. 
+  rewrite H4 in H3. eapply uniqueMid in H3. split. intros c. apply H. 
+  invIn; solveIn. split. intros c. apply H1. invIn; solveIn. intros c. 
+  apply H3. invIn; solveIn. 
+Qed. 
+
 Theorem TripleNeq : forall (A:Type) (u1 u2 u3:A) U D1 D2 D3 D4, 
                       genericUnique U (fun x => x) (D1++u1::D2++u2::D3++u3::D4) ->
                       u1 <> u2 /\ u2 <> u3 /\ u1 <> u3. 
 Proof.
   intros. assert(D1++u1::D2++u2::D3++u3::D4 = (D1++[u1]) ++ (D2++u2::D3++u3::D4)). 
-  rewrite <- app_assoc. simpl. auto. copy H. rewrite H0 in H. eapply uniqueAppendNeq in H. 
-  Focus 2. apply in_app_iff. right. simpl. eauto. Focus 2. rewrite in_app_iff. 
-  simpl. right. left. auto. split. auto. 
+  rewrite <- app_assoc. simpl. auto. copy H. rewrite H0 in H. 
+  eapply uniqueAppendNeq in H. Focus 2. apply in_app_iff. right. simpl. eauto. 
+  Focus 2. rewrite in_app_iff. simpl. right. left. auto. split. auto. 
   assert(D1++u1::D2++u2::D3++u3::D4 = (D1++u1::D2++u2::D3)++(u3::D4)). 
   repeat rewrite <- app_assoc. simpl. rewrite <- app_assoc. simpl. auto. 
-  copy H1. rewrite H2 in H1. eapply uniqueAppendNeq in H1. Focus 2. rewrite in_app_iff. 
-  right. simpl. right. rewrite in_app_iff. right. simpl. auto. Focus 2. simpl. auto. 
-  split; auto. assert(D1++u1::D2++u2::D3++u3::D4 = (D1++[u1]) ++ (D2++u2::D3++u3::D4)). 
-  rewrite <- app_assoc. auto. rewrite H4 in H3. eapply uniqueAppendNeq in H3. Focus 2. 
-  rewrite in_app_iff. right. simpl. auto. Focus 2. rewrite in_app_iff. simpl. 
-  right. right. rewrite in_app_iff. simpl. right. left. auto. auto. 
+  copy H1. rewrite H2 in H1. eapply uniqueAppendNeq in H1. Focus 2.
+  rewrite in_app_iff. right. simpl. right. rewrite in_app_iff. right. simpl. auto. 
+  Focus 2. simpl. auto. split; auto.
+  assert(D1++u1::D2++u2::D3++u3::D4 = (D1++[u1]) ++ (D2++u2::D3++u3::D4)). 
+  rewrite <- app_assoc. auto. rewrite H4 in H3. eapply uniqueAppendNeq in H3. 
+  Focus 2. rewrite in_app_iff. right. simpl. auto. Focus 2. rewrite in_app_iff. 
+  simpl. right. right. rewrite in_app_iff. simpl. right. left. auto. auto. 
 Qed. 
 
-Ltac solveIn :=
-  match goal with
-      | |- In ?x (?a ++ ?b) => rewrite in_app_iff; simpl; solve[left; solveIn|right; solveIn]
-      | |- In ?a ?b \/ In ?c ?d => solve[left; solveIn | right; solveIn]
-      | |- _ => eauto
-  end. 
+Theorem color_convert_base : forall Gamma Delta c u eta' eta'' G C eta, 
+                               convert_base Gamma Delta c G ->
+                               ~ In u Delta -> u < C ->
+                               setVertices Gamma C 0 eta' eta -> 
+                               coloring (eta'++(c,u)::eta'') G C. 
+Proof.
+  intros. induction H. 
+  {constructor. }
+  {eapply V_V'MapToUOrC in H; eauto. inv H. 
+   {invertHyp. econstructor. solveIn. solveIn. omega. omega. intros c. subst. apply H0. 
+    solveIn. econstructor. solveIn. solveIn. omega. omega. omega. apply IHconvert_base; auto. 
+    intros c. apply H0. solveIn. }
+   {invertHyp. econstructor. solveIn. solveIn. omega. omega. omega. econstructor. solveIn. 
+    solveIn. omega. omega. intros c. apply H0. solveIn. apply IHconvert_base; auto. 
+    intros c. apply H0. solveIn. }
+  }
+Qed. 
 
 Theorem convFormulaColorable : forall i Gamma Delta G eta K U eta'' F eta' C, 
                                  setVertices Gamma C 0 eta' eta -> SAT' eta (F::K) ->
@@ -163,73 +204,242 @@ Theorem convFormulaColorable : forall i Gamma Delta G eta K U eta'' F eta' C,
                                  convFormula i Gamma Delta F G -> coloring (eta'++eta'') G C.
 Proof. 
   intros. inv H3. simpl. destruct e1. destruct e2. destruct e3. simpl in H2. 
-  copy H2. apply TripleNeq in H2. invertHyp. inv H1.  
-  {inv H21. 
-   {copy H. eapply InTrueV in H; eauto. invertHyp. subst. inv H8. copy H10.
-    eapply InTrueV' in H10; eauto. econstructor; try apply in_app_iff; simpl; eauto; try omega.  
-    inv H12. 
+  copy H2. apply TripleNeq in H2. invertHyp. copy H3.
+  eapply TripleNotIn in H10. invertHyp. inv H1. 
+  {inv H23.  
+   {copy H. eapply InTrueV in H; eauto. invertHyp. subst. inv H8. copy H15.
+    econstructor; try apply in_app_iff; simpl; eauto; try omega. inv H12. 
     {eapply V_V'MapToUOrC in H5; eauto. inv H5. 
      {invertHyp. econstructor. solveIn. solveIn. omega. auto. omega. copy H. 
-      eapply V_V'MapToUOrC in H6; eauto. inv H6; invertHyp. 
-      {inv H13; econstructor; try solveIn; try omega. 
-
-
-admit. admit. }
-      {inv H13; econstructor; try solveIn; try omega. admit. admit. }
+      eapply V_V'MapToUOrC in H6; eauto. inv H6; invertHyp.  
+      {inv H13; econstructor; try solveIn; try omega; eapply color_convert_base; eauto. }
+      {inv H13; econstructor; try solveIn; try omega; eapply color_convert_base; eauto. }
      }
-      
+     {invertHyp. econstructor. solveIn. solveIn. omega. simpl in *. omega. auto. copy H6.
+      eapply V_V'MapToUOrC in H6; eauto. inv H6; invertHyp. 
+      {inv H13; econstructor; try solveIn; try omega; eapply color_convert_base; eauto. }
+      {inv H13; econstructor; try solveIn; try omega; eapply color_convert_base; eauto. }
+     }
+    }
+    {eapply V_V'MapToUOrC in H5; eauto. inv H5. 
+     {invertHyp. econstructor. solveIn. solveIn. omega. simpl in *. omega. auto. 
+      eapply V_V'MapToUOrC in H6; eauto. inv H6; invertHyp.  
+      {inv H13; econstructor; try solveIn; try omega; eapply color_convert_base; eauto. }
+      {inv H13; econstructor; try solveIn; try omega; eapply color_convert_base; eauto. }
+     }
+     {invertHyp. econstructor. solveIn. solveIn. omega. simpl in *. omega. omega. copy H6.
+      eapply V_V'MapToUOrC in H6; eauto. inv H6; invertHyp. 
+      {inv H13; econstructor; try solveIn; try omega; eapply color_convert_base; eauto. }
+      {inv H13; econstructor; try solveIn; try omega; eapply color_convert_base; eauto. }
+     }
+    }
+   }
+   {copy H. eapply InFalseV in H; eauto. invertHyp. subst. inv H8. copy H15.
+    econstructor; try apply in_app_iff; simpl; eauto; try omega. inv H12. 
+    {eapply V_V'MapToUOrC in H5; eauto. inv H5. 
+     {invertHyp. econstructor. solveIn. solveIn. omega. auto. omega. copy H. 
+      eapply V_V'MapToUOrC in H6; eauto. inv H6; invertHyp.  
+      {inv H13; econstructor; try solveIn; try omega; eapply color_convert_base; eauto. }
+      {inv H13; econstructor; try solveIn; try omega; eapply color_convert_base; eauto. }
+     }
+     {invertHyp. econstructor. solveIn. solveIn. omega. simpl in *. omega. auto. copy H6.
+      eapply V_V'MapToUOrC in H6; eauto. inv H6; invertHyp. 
+      {inv H13; econstructor; try solveIn; try omega; eapply color_convert_base; eauto. }
+      {inv H13; econstructor; try solveIn; try omega; eapply color_convert_base; eauto. }
+     }
+    }
+    {eapply V_V'MapToUOrC in H5; eauto. inv H5. 
+     {invertHyp. econstructor. solveIn. solveIn. omega. simpl in *. omega. auto. 
+      eapply V_V'MapToUOrC in H6; eauto. inv H6; invertHyp.  
+      {inv H13; econstructor; try solveIn; try omega; eapply color_convert_base; eauto. }
+      {inv H13; econstructor; try solveIn; try omega; eapply color_convert_base; eauto. }
+     }
+     {invertHyp. econstructor. solveIn. solveIn. omega. simpl in *. omega. omega. copy H6.
+      eapply V_V'MapToUOrC in H6; eauto. inv H6; invertHyp. 
+      {inv H13; econstructor; try solveIn; try omega; eapply color_convert_base; eauto. }
+      {inv H13; econstructor; try solveIn; try omega; eapply color_convert_base; eauto. }
+     }
+    }
+   }
+  }
+  {inv H23.   
+   {copy H. eapply InTrueV in H; eauto. invertHyp. subst.
+    eapply V_V'MapToUOrC in H4; eauto. inv H4; invertHyp. 
+    {inv H8; econstructor; try solveIn; try omega. 
+     {inv H12; econstructor; try solveIn; try omega. 
+      {eapply V_V'MapToUOrC in H6; eauto. inv H6; invertHyp.  
+       {inv H13;econstructor; try solveIn; try omega; eapply color_convert_base; eauto. }
+       {inv H13;econstructor; try solveIn; try omega; eapply color_convert_base; eauto. }
+      }
+     }
+     {inv H12; econstructor; try solveIn; try omega. 
+      {eapply V_V'MapToUOrC in H6; eauto. inv H6; invertHyp.  
+       {inv H13; econstructor; try solveIn; try omega; eapply color_convert_base; eauto. }
+       {inv H13; econstructor; try solveIn; try omega; eapply color_convert_base; eauto. }
+      }
+     }
+    }
+    {inv H8; econstructor; try solveIn; try omega. 
+     {inv H12; econstructor; try solveIn; try omega. 
+      {eapply V_V'MapToUOrC in H6; eauto. inv H6; invertHyp.  
+       {inv H13; econstructor; try solveIn; try omega; eapply color_convert_base; eauto. }
+       {inv H13; econstructor; try solveIn; try omega; eapply color_convert_base; eauto. }
+      }
+     }
+     {inv H12; econstructor; try solveIn; try omega. 
+      {eapply V_V'MapToUOrC in H6; eauto. inv H6; invertHyp.  
+       {inv H13; econstructor; try solveIn; try omega; eapply color_convert_base; eauto. }
+       {inv H13; econstructor; try solveIn; try omega; eapply color_convert_base; eauto. }
+      }
+     }
+    }
+   }
+   {copy H. eapply InFalseV in H; eauto. invertHyp. subst.
+    eapply V_V'MapToUOrC in H4; eauto. inv H4; invertHyp. 
+    {inv H8; econstructor; try solveIn; try omega. 
+     {inv H12; econstructor; try solveIn; try omega. 
+      {eapply V_V'MapToUOrC in H6; eauto. inv H6; invertHyp.  
+       {inv H13; econstructor; try solveIn; try omega; eapply color_convert_base; eauto.  }
+       {inv H13; econstructor; try solveIn; try omega; eapply color_convert_base; eauto. }
+      }
+     }
+     {inv H12; econstructor; try solveIn; try omega. 
+      {eapply V_V'MapToUOrC in H6; eauto. inv H6; invertHyp.  
+       {inv H13; econstructor; try solveIn; try omega; eapply color_convert_base; eauto. }
+       {inv H13; econstructor; try solveIn; try omega; eapply color_convert_base; eauto. }
+      }
+     }
+    }
+    {inv H8; econstructor; try solveIn; try omega. 
+     {inv H12; econstructor; try solveIn; try omega. 
+      {eapply V_V'MapToUOrC in H6; eauto. inv H6; invertHyp.  
+       {inv H13; econstructor; try solveIn; try omega; eapply color_convert_base; eauto. }
+       {inv H13; econstructor; try solveIn; try omega; eapply color_convert_base; eauto. }
+      }
+     }
+     {inv H12; econstructor; try solveIn; try omega. 
+      {eapply V_V'MapToUOrC in H6; eauto. inv H6; invertHyp.  
+       {inv H13; econstructor; try solveIn; try omega; eapply color_convert_base; eauto. }
+       {inv H13; econstructor; try solveIn; try omega; eapply color_convert_base; eauto. }
+      }
+     }
+    }
+   } 
+  }
+  {inv H23.   
+   {copy H. eapply InTrueV in H; eauto. invertHyp. subst.
+    eapply V_V'MapToUOrC in H4; eauto. inv H4; invertHyp. 
+    {inv H8; econstructor; try solveIn; try omega. 
+     {eapply V_V'MapToUOrC in H5; eauto. inv H5; invertHyp. 
+      {inv H12; econstructor; try solveIn; try omega. 
+       {inv H13; econstructor; try solveIn; try omega;eapply color_convert_base; eauto. }
+       {inv H13; econstructor; try solveIn; try omega;eapply color_convert_base; eauto. }
+      }
+      {inv H12; econstructor; try solveIn; try omega. 
+       {inv H13; econstructor; try solveIn; try omega;eapply color_convert_base; eauto. }
+       {inv H13; econstructor; try solveIn; try omega;eapply color_convert_base; eauto. }
+      }
+     }
+     {eapply V_V'MapToUOrC in H5; eauto. inv H5; invertHyp. 
+      {inv H12; econstructor; try solveIn; try omega. 
+       {inv H13; econstructor; try solveIn; try omega;eapply color_convert_base; eauto. }
+       {inv H13; econstructor; try solveIn; try omega;eapply color_convert_base; eauto. }
+      }
+      {inv H12; econstructor; try solveIn; try omega. 
+       {inv H13; econstructor; try solveIn; try omega;eapply color_convert_base; eauto. }
+       {inv H13; econstructor; try solveIn; try omega;eapply color_convert_base; eauto. }
+      }
+     }
+    }
+    {inv H8; econstructor; try solveIn; try omega. 
+     {eapply V_V'MapToUOrC in H5; eauto. inv H5; invertHyp. 
+      {inv H12; econstructor; try solveIn; try omega. 
+       {inv H13; econstructor; try solveIn; try omega;eapply color_convert_base; eauto. }
+       {inv H13; econstructor; try solveIn; try omega;eapply color_convert_base; eauto. }
+      }
+      {inv H12; econstructor; try solveIn; try omega. 
+       {inv H13; econstructor; try solveIn; try omega;eapply color_convert_base; eauto. }
+       {inv H13; econstructor; try solveIn; try omega;eapply color_convert_base; eauto. }
+      }
+     }
+     {eapply V_V'MapToUOrC in H5; eauto. inv H5; invertHyp. 
+      {inv H12; econstructor; try solveIn; try omega. 
+       {inv H13; econstructor; try solveIn; try omega;eapply color_convert_base; eauto. }
+       {inv H13; econstructor; try solveIn; try omega;eapply color_convert_base; eauto. }
+      }
+      {inv H12; econstructor; try solveIn; try omega. 
+       {inv H13; econstructor; try solveIn; try omega;eapply color_convert_base; eauto. }
+       {inv H13; econstructor; try solveIn; try omega;eapply color_convert_base; eauto. }
+      }
+     }
+    }
+   }
+   {copy H. eapply InFalseV in H; eauto. invertHyp. subst.
+    eapply V_V'MapToUOrC in H4; eauto. inv H4; invertHyp. 
+    {inv H8; econstructor; try solveIn; try omega. 
+     {eapply V_V'MapToUOrC in H5; eauto. inv H5; invertHyp. 
+      {inv H12; econstructor; try solveIn; try omega. 
+       {inv H13; econstructor; try solveIn; try omega;eapply color_convert_base; eauto. }
+       {inv H13; econstructor; try solveIn; try omega;eapply color_convert_base; eauto. }
+      }
+      {inv H12; econstructor; try solveIn; try omega. 
+       {inv H13; econstructor; try solveIn; try omega;eapply color_convert_base; eauto. }
+       {inv H13; econstructor; try solveIn; try omega;eapply color_convert_base; eauto. }
+      }
+     }
+     {eapply V_V'MapToUOrC in H5; eauto. inv H5; invertHyp. 
+      {inv H12; econstructor; try solveIn; try omega. 
+       {inv H13; econstructor; try solveIn; try omega;eapply color_convert_base; eauto. }
+       {inv H13; econstructor; try solveIn; try omega;eapply color_convert_base; eauto. }
+      }
+      {inv H12; econstructor; try solveIn; try omega. 
+       {inv H13; econstructor; try solveIn; try omega;eapply color_convert_base; eauto. }
+       {inv H13; econstructor; try solveIn; try omega;eapply color_convert_base; eauto. }
+      }
+     }
+    }
+    {inv H8; econstructor; try solveIn; try omega. 
+     {eapply V_V'MapToUOrC in H5; eauto. inv H5; invertHyp. 
+      {inv H12; econstructor; try solveIn; try omega. 
+       {inv H13; econstructor; try solveIn; try omega;eapply color_convert_base; eauto. }
+       {inv H13; econstructor; try solveIn; try omega;eapply color_convert_base; eauto. }
+      }
+      {inv H12; econstructor; try solveIn; try omega. 
+       {inv H13; econstructor; try solveIn; try omega;eapply color_convert_base; eauto. }
+       {inv H13; econstructor; try solveIn; try omega;eapply color_convert_base; eauto. }
+      }
+     }
+     {eapply V_V'MapToUOrC in H5; eauto. inv H5; invertHyp. 
+      {inv H12; econstructor; try solveIn; try omega. 
+       {inv H13; econstructor; try solveIn; try omega;eapply color_convert_base; eauto. }
+       {inv H13; econstructor; try solveIn; try omega;eapply color_convert_base; eauto. }
+      }
+      {inv H12; econstructor; try solveIn; try omega. 
+       {inv H13; econstructor; try solveIn; try omega;eapply color_convert_base; eauto. }
+       {inv H13; econstructor; try solveIn; try omega;eapply color_convert_base; eauto. }
+      }
+     }
+    }
+   }
+  }
+Qed. 
 
- copy H. eapply InNeq in H; eauto. invertHyp. econstructor. apply in_app_iff.
-     simpl. auto. apply in_app_iff. simpl. eauto. auto. auto. auto. 
-     inv H12. 
-
-
-inversion H8; subst. 
-    {inversion H12; subst.  
-     {inversion H13; subst. 
-      {inv H18. copy H3. eapply InEtaInEta' in H1; eauto. inv H1. invertHyp. 
-       eapply 
-
-simpl in *. 
-    {eapply helper; eauto. simpl. eauto. eapply helper; eauto. simpl. eauto. simpl.
-     
-
-
-
-inv H18.  
-     {copy H4. eapply V_V'MapToUOrC in H4; try eassumption. inv H4. 
-      {invertHyp. inv H0. eapply lookupEta'Det in H17; eauto. subst. econstructor. 
-       apply in_app_iff. simpl. right. eauto. apply in_app_iff. left. eauto. omega. 
-       auto. omega. 
-
-
- copy H3. eapply InEtaInEta' in H3; eauto. inv H3. 
-       {invertHyp. econstructor. apply in_app_iff. right. simpl. eauto. apply in_app_iff. 
-        left. eauto. 
-
-Focus 2. 
-       invertHyp. econstructor. apply in_app_iff. right. simpl. eauto. apply in_app_iff.
-       left. eauto. auto. omega. omega. omega. 
-
-
-
-Theorem A : forall Gamma u C eta eta', 
-              setVertices Gamma C 0 eta' eta -> In (u,3*u,3*u+1,3*u+2) Gamma ->
-              coloring
-
-Theorem convStackColorable : forall i Gamma Delta G eta F j S5 eta'' eta' C, 
-                               setVertices Gamma C 0 eta' eta -> 
-                               setCs eta' j F eta'' eta ->
+Theorem convStackColorable : forall i Gamma Delta G eta F S5 eta'' eta' C, 
+                               setVertices Gamma C 0 eta' eta -> SAT' eta F ->
+                               setCs eta' i F eta'' eta ->
                                genericUnique S5 (fun x => x) Delta -> 
                                convStack i Gamma Delta F G -> coloring (eta' ++ eta'') G C.
 Proof.
-  intros. genDeps {{ S5; eta; eta'; C; eta''; j }}. induction H2; intros. 
+  intros. genDeps {{ S5; eta; eta'; C; eta'' }}. induction H3; intros. 
   {constructor. }
   {constructor. 
-   {inv H1. 
-    {rewrite consApp. apply colorWeakeningApp. eapply IHconvStack; eauto. }
-    {rewrite consApp. apply colorWeakeningApp. eapply IHconvStack; eauto. }
-    {rewrite consApp. apply colorWeakeningApp. eapply IHconvStack; eauto. }
+   {inv H1. inv H2. 
+    {rewrite consApp. apply colorWeakeningApp. eapply IHconvStack; eauto. 
+     rewrite plus_comm. auto. }
+    {rewrite consApp. apply colorWeakeningApp. eapply IHconvStack; eauto.
+     rewrite plus_comm. auto. }
+    {rewrite consApp. apply colorWeakeningApp. eapply IHconvStack; eauto.
+     rewrite plus_comm. auto. }
    }
    {eapply convFormulaColorable; eauto. }
   }
@@ -265,8 +475,4 @@ Qed.
 
 
 
-
-
-
-ad;lfkhjasdf
 
