current/colorImpliesSAT.v
@@ -1,0 +1,60 @@
+Require Import ThreeSatReduction.  
+
+
+
+
+Theorem convStackOutOfScope : forall eta'' eta' i Gamma Delta K G j c C eta, 
+                                convStack i Gamma Delta K G ->j < i -> 
+                                setVertices Gamma C 0 eta' eta -> setCs eta' i K eta'' eta ->
+                                coloring (eta'++(j,c)::eta'') G C ->
+                                coloring (eta'++eta'') G C. 
+Proof.
+  intros. genDeps {{ eta; eta'; eta''; j; C; c }}. induction H; intros. 
+  {constructor. }
+  {constructor. 
+
+
+Fixpoint graphFVs G :=
+  match G with
+    |emptyGraph => []
+    |newEdge u v G => u::v::graphFVs G
+    |gunion G1 G2 => graphFVs G1 ++ graphFVs G2
+  end.
+
+Theorem colorImpliesSATFormula : forall Gamma C eta eta' i U eta'' Delta F G,
+                            setVertices Gamma C 0 eta' eta -> setCs eta' i F eta'' eta ->
+                            coloring (eta'++eta'') G C -> i >= 3 * length Gamma ->
+                            genericUnique U (fun x => x) Delta -> 
+                            convStack i Gamma Delta F G -> SAT' eta F. 
+Proof.
+  intros. genDeps {{ U; eta; eta'; eta''; C }}. induction H4; intros. 
+  {constructor. } 
+  {destruct F. destruct p. inv H3. 
+   {inv H13. 
+    {constructor. left. constructor. auto. eapply IHconvStack. omega. Focus 3.
+     rewrite plus_comm. eauto. Focus 3. eauto. Focus 2. eauto. 
+
+
+ 
+
+     eapply convStackOutOfScope. eauto. Focus 2. eauto. Focus 2. rewrite plus_comm. 
+     eauto. Focus 2. inv H1. eauto. omega. }
+    {constructor. left. constructor. auto. eapply IHconvStack. Focus 3.
+     rewrite plus_comm. eauto. Focus 3. eauto. Focus 2. eauto. admit. }
+   }
+   {inv H12. 
+    {constructor. right. left. constructor. auto. eapply IHconvStack. Focus 3.
+     rewrite plus_comm. eauto. Focus 3. eauto. Focus 2. eauto. admit. }
+    {constructor. right. left. constructor. auto. eapply IHconvStack. Focus 3.
+     rewrite plus_comm. eauto. Focus 3. eauto. Focus 2. eauto. admit. }
+   }
+   {inv H12. 
+    {constructor. right. right. constructor. auto. eapply IHconvStack. Focus 3.
+     rewrite plus_comm. eauto. Focus 3. eauto. Focus 2. eauto. admit. }
+    {constructor. right. right. constructor. auto. eapply IHconvStack. Focus 3.
+     rewrite plus_comm. eauto. Focus 3. eauto. Focus 2. eauto. admit. }
+   }
+  }
+Qed. 
+
+
